src/Ex/Msi/MsiObjInv.v
@@ -1,0 +1,92 @@
+Require Import Bool List String Peano_dec Lia.
+Require Import Common FMap IndexSupport HVector Syntax Topology Semantics SemFacts StepM.
+Require Import Invariant TrsInv Simulation Serial SerialFacts.
+Require Import RqRsLangEx RqRsCorrect.
+
+Require Import Ex.Spec Ex.SpecInds Ex.Template.
+Require Import Ex.Msi Ex.Msi.Msi.
+
+Set Implicit Arguments.
+
+Import PropMonadNotations.
+Import CaseNotations.
+
+Local Open Scope list.
+Local Open Scope hvec.
+Local Open Scope fmap.
+
+Existing Instance Msi.ImplOStateIfc.
+
+Section ObjInv.
+  Variable topo: DTree.
+
+  Definition MsiUpLockObjInv (oidx: IdxT): ObjInv :=
+    fun ost orq =>
+      (rqiu <+- orq@[upRq];
+      rmsg <+- rqiu.(rqi_msg);
+      match case rmsg.(msg_id) on idx_dec default True with
+      | msiRqS:
+          ost#[owned] = false /\ ost#[status] <= msiI /\
+          ost#[dir].(dir_st) <= msiS
+      | msiRqM:
+          ost#[owned] = false /\ ost#[status] <= msiS /\
+          ost#[dir].(dir_st) <= msiS
+      end).
+
+  Definition DownLockFromChild (oidx: IdxT) (rqid: RqInfo Msg) :=
+    exists cidx,
+      rqid.(rqi_midx_rsb) = Some (downTo cidx) /\
+      parentIdxOf topo cidx = Some oidx.
+
+  Definition DownLockFromParent (oidx: IdxT) (rqid: RqInfo Msg) :=
+    rqid.(rqi_midx_rsb) = Some (rsUpFrom oidx).
+
+  Definition MsiDownLockObjInv (oidx: IdxT): ObjInv :=
+    fun ost orq =>
+      (rqid <+- orq@[downRq];
+      rmsg <+- rqid.(rqi_msg);
+      match case rmsg.(msg_id) on idx_dec default True with
+      | msiRqS: DownLockFromChild oidx rqid /\
+                ost#[status] <= msiI /\ ost#[dir].(dir_st) = msiM /\
+                In ost#[dir].(dir_excl) (subtreeChildrenIndsOf topo oidx) /\
+                rqid.(rqi_minds_rss) = [rsUpFrom ost#[dir].(dir_excl)]
+      | msiRqM: DownLockFromChild oidx rqid /\
+                ost#[status] <= msiS /\
+                ((ost#[owned] = true /\ ost#[dir].(dir_st) = msiS /\
+                  SubList ost#[dir].(dir_sharers) (subtreeChildrenIndsOf topo oidx) /\
+                  rqid.(rqi_minds_rss) = map rsUpFrom ost#[dir].(dir_sharers)) \/
+                 (ost#[dir].(dir_st) = msiM /\
+                  In ost#[dir].(dir_excl) (subtreeChildrenIndsOf topo oidx) /\
+                  rqid.(rqi_minds_rss) = [rsUpFrom ost#[dir].(dir_excl)]))
+      | msiDownRqS: DownLockFromParent oidx rqid /\
+                    ost#[status] <= msiI /\ ost#[dir].(dir_st) = msiM /\
+                    In ost#[dir].(dir_excl) (subtreeChildrenIndsOf topo oidx) /\
+                    rqid.(rqi_minds_rss) = [rsUpFrom ost#[dir].(dir_excl)]
+      | msiDownRqI: DownLockFromParent oidx rqid /\
+                    ((ost#[dir].(dir_st) = msiS /\
+                      SubList ost#[dir].(dir_sharers) (subtreeChildrenIndsOf topo oidx) /\
+                      rqid.(rqi_minds_rss) = map rsUpFrom ost#[dir].(dir_sharers)) \/
+                     (ost#[dir].(dir_st) = msiM /\
+                      In ost#[dir].(dir_excl) (subtreeChildrenIndsOf topo oidx) /\
+                      rqid.(rqi_minds_rss) = [rsUpFrom ost#[dir].(dir_excl)]))
+      end).
+
+  Definition MsiObjInvs (oidx: IdxT): ObjInv :=
+    fun ost orq =>
+      MsiUpLockObjInv oidx ost orq /\
+      MsiDownLockObjInv oidx ost orq.
+
+End ObjInv.
+
+Ltac disc_msi_obj_invs :=
+  repeat
+    match goal with
+    | [H: MsiObjInvs _ _ _ _ |- _] => destruct H
+    | [H: MsiUpLockObjInv _ _ _ |- _] =>
+      red in H; mred; simpl in H; disc_rule_conds_const
+    | [H: MsiDownLockObjInv _ _ _ _ |- _] =>
+      red in H; mred; simpl in H; disc_rule_conds_const
+    | [Hmsg: msg_id ?rmsg = _, H: context [msg_id ?rmsg] |- _] =>
+      rewrite Hmsg in H; simpl in H
+    end.
+
