src/Ex/Msi/MsiTopo.v
@@ -1,10 +1,10 @@
 Require Import Bool Vector List String Peano_dec Omega.
 Require Import Common FMap HVector ListSupport IndexSupport.
-Require Import Syntax Topology Semantics.
+Require Import Syntax Topology Semantics Invariant.
 Require Import RqRsLangEx.
 
 Require Import Ex.Spec Ex.SpecInds Ex.Template Ex.Msi.
-Require Import Ex.Msi.Msi.
+Require Import Ex.Msi.Msi Ex.Msi.MsiObjInv.
 
 Set Implicit Arguments.
 
@@ -409,11 +409,13 @@ Section System.
       end
     end.
 
-  Lemma msi_RqUpRsUpOkSys: RqUpRsUpOkSys topo impl.
+  Ltac disc_rule_custom ::= disc_msi_obj_invs.
+  
+  Lemma msi_RqUpRsUpOkSys: RqUpRsUpOkSys topo impl (MsiObjInvs topo).
   Proof. (* SKIP_PROOF_OFF *)
     repeat
       match goal with
-      | |- RqUpRsUpOkSys _ _ => red
+      | |- RqUpRsUpOkSys _ _ _ => red
       | |- Forall _ _ => simpl; constructor; simpl
       | |- Forall _ (_ ++ _) => apply Forall_app
       end.
@@ -446,15 +448,39 @@ Section System.
            apply in_map_iff in H; dest; subst;
            dest_in|dest_in].
         all: try (exfalso_RsToUpRule; fail).
-        all: try (clear; solve_rule_conds_ex; solve_msi).
-        { clear; solve_rule_conds_const.
-          all: try (destruct H6; dest; try solve [congruence|solve_msi]).
+        { clear; solve_rule_conds_ex; solve_msi. }
+        { clear; solve_rule_conds_ex; solve_msi. }
+        { clear; solve_rule_conds_ex; solve_msi. }
+        { clear; solve_rule_conds_ex.
+          { destruct H17; dest; try solve [congruence|solve_msi]. }
+          { destruct H17; dest; try solve [congruence|solve_msi]. }
+        }          
+        { clear; solve_rule_conds_ex; solve_msi. }
+        { clear; solve_rule_conds_ex.
+          { destruct H16; dest; try solve [congruence|solve_msi]. }
+          { destruct H16; dest; try solve [congruence|solve_msi].
+            f_equal; apply M.add_remove_comm; discriminate.
+          }
+        }           
+
+      + simpl in H2; apply in_app_or in H2; destruct H2;
+          [unfold liRulesFromChildren in H;
+           apply concat_In in H; dest;
+           apply in_map_iff in H; dest; subst;
+           dest_in|dest_in].
+        all: try (exfalso_RsToUpRule; fail).
+
+        { clear; solve_rule_conds_ex; solve_msi. }
+        { clear; solve_rule_conds_ex; solve_msi. }
+        { clear; solve_rule_conds_ex; solve_msi. }
+        { clear; solve_rule_conds_ex.
+          all: try (destruct H17; dest; try solve [congruence|solve_msi]).
         }
-        { clear; solve_rule_conds_const.
-          { mred; rewrite Hmsg; simpl; split; [assumption|congruence]. }
-          { mred; rewrite Hidx; simpl; auto. }
-          { mred; simpl; rewrite Hmsg, Hidx; simpl.
-            repeat split; auto; simpl; try solve [mred|solve_msi].
+        { clear; solve_rule_conds_ex; solve_msi. }
+        { clear; solve_rule_conds_ex.
+          { destruct H16; dest; try solve [congruence|solve_msi]. }
+          { destruct H16; dest; try solve [congruence|solve_msi]. }
+          { destruct H16; dest; try solve [congruence|solve_msi].
             f_equal; apply M.add_remove_comm; discriminate.
           }
         }
@@ -465,46 +491,17 @@ Section System.
            apply in_map_iff in H; dest; subst;
            dest_in|dest_in].
         all: try (exfalso_RsToUpRule; fail).
-        all: try (clear; solve_rule_conds_ex; solve_msi).
-        { clear; solve_rule_conds_const.
-          all: try (destruct H6; dest; try solve [congruence|solve_msi]).
-        }
-        { clear; solve_rule_conds_const.
-          { mred; rewrite Hmsg; simpl; split; [assumption|congruence]. }
-          { mred; rewrite Hidx; simpl; auto. }
-          { mred; simpl; rewrite Hmsg, Hidx; simpl.
-            repeat split; auto; simpl; try solve [mred|solve_msi].
-            f_equal; apply M.add_remove_comm; discriminate.
-          }
-        }
 
-      + simpl in H2; apply in_app_or in H2; destruct H2;
-          [unfold liRulesFromChildren in H;
-           apply concat_In in H; dest;
-           apply in_map_iff in H; dest; subst;
-           dest_in|dest_in].
-        all: try (exfalso_RsToUpRule; fail).
-        all: try (clear; solve_rule_conds_ex; solve_msi).
+        { clear; solve_rule_conds_ex; solve_msi. }
         { clear; solve_rule_conds_const; try solve_msi.
-          unfold addRqS in H0; mred.
+          unfold addRqS in H1; mred.
         }
+        { clear; solve_rule_conds_ex; solve_msi. }
+        { clear; solve_rule_conds_ex; solve_msi. }
         { clear; solve_rule_conds_const; try solve_msi.
-          unfold addRqS in H0; mred.
+          unfold addRqS in H1; mred.
         }
-        { clear; solve_rule_conds_const.
-          { unfold addRqS in Hrqi; mred. }
-          { unfold addRqS in Hrqi; mred.
-            rewrite Hmsg; simpl; split; [assumption|congruence].
-          }
-          { unfold addRqS in Hrqi; mred.
-            mred; rewrite Hidx; simpl; auto.
-          }
-          { unfold addRqS in Hrqi; mred.
-            simpl; rewrite Hmsg, Hidx; simpl.
-            repeat split; auto; simpl; try solve [mred|solve_msi].
-            f_equal; apply M.add_remove_comm; discriminate.
-          }
-        }
+        { clear; solve_rule_conds_ex; solve_msi. }
         
       + simpl in H2; apply in_app_or in H2; destruct H2;
           [unfold liRulesFromChildren in H;
@@ -512,27 +509,17 @@ Section System.
            apply in_map_iff in H; dest; subst;
            dest_in|dest_in].
         all: try (exfalso_RsToUpRule; fail).
-        all: try (clear; solve_rule_conds_ex; solve_msi).
+        
+        { clear; solve_rule_conds_ex; solve_msi. }
         { clear; solve_rule_conds_const; try intuition solve_msi.
-          unfold addRqS in H0; mred.
+          unfold addRqS in H1; mred.
         }
+        { clear; solve_rule_conds_ex; solve_msi. }
+        { clear; solve_rule_conds_ex; solve_msi. }
         { clear; solve_rule_conds_const; try intuition solve_msi.
-          unfold addRqS in H0; mred.
+          unfold addRqS in H1; mred.
         }
-        { clear; solve_rule_conds_const; try intuition solve_msi.
-          { unfold addRqS in Hrqi; mred. }
-          { unfold addRqS in Hrqi; mred.
-            rewrite Hmsg; simpl; split; [assumption|congruence].
-          }
-          { unfold addRqS in Hrqi; mred.
-            mred; rewrite Hidx; simpl; auto.
-          }
-          { unfold addRqS in Hrqi; mred.
-            simpl; rewrite Hmsg, Hidx; simpl.
-            repeat split; auto; simpl; try solve [mred|intuition solve_msi].
-            f_equal; apply M.add_remove_comm; discriminate.
-          }
-        }
+        { clear; solve_rule_conds_ex; solve_msi. }
 
     - (** L1 cache *)
       apply Forall_forall; intros.
@@ -556,19 +543,19 @@ Section System.
       + preveal H4; dest_in.
         all: try (exfalso_RsToUpRule; fail).
         { clear; solve_rule_conds_const; try solve_msi.
-          unfold addRqS in H0; mred.
+          unfold addRqS in H1; mred.
         }
         { clear; solve_rule_conds_const; try solve_msi.
-          unfold addRqS in H0; mred.
+          unfold addRqS in H1; mred.
         }
 
       + preveal H4; dest_in.
         all: try (exfalso_RsToUpRule; fail).
         { clear; solve_rule_conds_const; try solve_msi.
-          unfold addRqS in H0; mred.
+          unfold addRqS in H1; mred.
         }
         { clear; solve_rule_conds_const; try solve_msi.
-          unfold addRqS in H0; mred.
+          unfold addRqS in H1; mred.
         }
 
         (* END_SKIP_PROOF_OFF *)
@@ -669,14 +656,14 @@ Section System.
       (* END_SKIP_PROOF_OFF *)
   Qed.
 
-  Lemma msi_GoodRqRsInterfSys: GoodRqRsInterfSys topo impl.
+  Lemma msi_GoodRqRsInterfSys: GoodRqRsInterfSys topo impl (MsiObjInvs topo).
   Proof.
     split.
     - apply msi_RqUpRsUpOkSys.
     - apply msi_GoodExtRssSys.
   Qed.
 
-  Lemma msi_RqRsSys: RqRsSys topo impl.
+  Lemma msi_RqRsSys: RqRsSys topo impl (MsiObjInvs topo).
   Proof.
     red; repeat ssplit.
     - apply msi_RqRsDTree.
